Flapjack/Test/CompilerParity.lean
@@ -275,6 +275,7 @@ import Flapjack.Test.ParserKeepAnnotParity
 import Flapjack.Test.ParserTryProgParity
 import Flapjack.Test.ParserPancakePegParity
 import Flapjack.Test.ParserParseStatementParity
+import Flapjack.Test.ParserByteNamesParity
 import Flapjack.Test.PanLangWfShapeParity
 import Flapjack.Test.PanLangWfFieldsContextParity
 import Flapjack.Test.PanHHandleCallRetParity
